Add a FIFO module for debugging with an arbitrary size

Kami/Ex/Fifo.v
@@ -1,4 +1,5 @@
 Require Import Bool String List.
+Require Import Numbers.DecimalString.
 Require Import Lib.CommonTactics Lib.ilist Lib.Word Lib.Indexer Lib.StringAsList.
 Require Import Kami.Syntax Kami.Notations Kami.Semantics.
 Require Import Kami.Wf Kami.Tactics.
@@ -124,6 +125,83 @@ End DebugFifo.
 Hint Unfold debugFifo: ModuleDefs.
 Hint Unfold debugEnq debugDeq: MethDefs.
 
+Section DebugFifoN.
+  Variables (fifoName: string)
+            (sz: nat)
+            (dType: Kind)
+            (cntSz: nat).
+
+  Local Notation "^ s" := (fifoName -- s) (at level 0).
+
+  Variables (dmsg: string) (disp: forall ty, ty dType -> list (Disp ty)).
+
+  Definition debugEnqN {ty} : forall (d: ty dType), ActionT ty Void :=
+    fun d =>
+      (Read isFull <- ^"full";
+      Assert !#isFull;
+      Read eltT <- ^"elt";
+      Read enqPT <- ^"enqP";
+      Read deqPT <- ^"deqP";
+      Write ^"elt" <- #eltT@[#enqPT <- #d];
+      Write ^"empty" <- $$false;
+      LET next_enqP <- (#enqPT + $1) :: Bit sz;
+      Write ^"full" <- (#deqPT == #next_enqP);
+      Write ^"enqP" <- #next_enqP;
+      Retv)%kami_action.
+
+  Definition debugDeqN {ty} : ActionT ty dType :=
+    (Read isEmpty <- ^"empty";
+    Assert !#isEmpty;
+    Read eltT <- ^"elt";
+    Read enqPT <- ^"enqP";
+    Read deqPT <- ^"deqP";
+    Write ^"full" <- $$false;
+    LET next_deqP <- (#deqPT + $1) :: Bit sz;
+    Write ^"empty" <- (#enqPT == #next_deqP);
+    Write ^"deqP" <- #next_deqP;
+    Ret #eltT@[#deqPT])%kami_action.
+
+  Local Definition nat_to_string (n: nat): string :=
+    NilEmpty.string_of_uint (Nat.to_uint n).
+
+  Fixpoint displayN {ty} (elts: ty (Vector dType sz))
+           (n: nat) (cont: ActionT ty Void): ActionT ty Void :=
+    match n with
+    | O => cont
+    | S n' => (LET elt <- #elts@[$n'];
+              Display (dmsg ++ nat_to_string n')
+                      (disp _ elt) (displayN elts n' cont))%kami_action
+    end.
+
+  Definition debugCountN {ty}: ActionT ty Void :=
+    (Read countDone <- ^"countDone";
+    Assert !#countDone;
+    Read count: Bit cntSz <- ^"counter";
+    Write ^"counter" <- #count + $1;
+    Read isFull <- ^"full";
+    If (#count == $(Nat.pow 2 cntSz - 1) && #isFull)
+     then (Read elt: Vector dType sz <- ^"elt";
+          displayN elt (Nat.pow 2 sz) (Write ^"countDone" <- $$true; Retv));
+     Retv)%kami_action.
+
+  Definition debugFifoN := MODULE {
+    Register ^"elt" : Vector dType sz <- Default
+    with Register ^"enqP" : Bit sz <- Default
+    with Register ^"deqP" : Bit sz <- Default
+    with Register ^"empty" : Bool <- true
+    with Register ^"full" : Bool <- Default
+    with Register ^"countDone" : Bool <- Default
+    with Register ^"counter" : Bit cntSz <- Default
+    with Rule ^"count" := debugCountN
+    with Method ^"enq"(d : dType) : Void := (debugEnqN d)
+    with Method ^"deq"() : dType := debugDeqN
+  }.
+
+End DebugFifoN.
+
+Hint Unfold debugFifoN: ModuleDefs.
+Hint Unfold displayN debugEnqN debugDeqN: MethDefs.
+
 Section Facts.
   Variables (fifoName: string)
             (sz: nat)
@@ -158,12 +236,32 @@ Section Facts.
   Proof. kequiv. Qed.
   Hint Resolve debugFifo_ModEquiv.
 
+  Lemma debugFifoN_ModEquiv:
+    ModPhoasWf (debugFifoN fifoName sz cntSz dmsg disp).
+  Proof.
+    kequiv.
+    induction (Nat.pow 2 sz); simpl; kequiv.
+    assumption.
+  Qed.
+  Hint Resolve debugFifoN_ModEquiv.
+
   Lemma debugFifo_ValidRegs:
     ModRegsWf (debugFifo fifoName cntSz dmsg disp).
   Proof. kvr. Qed.
   Hint Resolve debugFifo_ValidRegs.
 
+  Lemma debugFifoN_ValidRegs:
+    ModRegsWf (debugFifoN fifoName sz cntSz dmsg disp).
+  Proof.
+    kvr.
+    induction (Nat.pow 2 sz); simpl; kvr.
+    assumption.
+  Qed.
+  Hint Resolve debugFifoN_ValidRegs.
+
 End Facts.
 
-Hint Resolve fifo_ModEquiv simpleFifo_ModEquiv.
-Hint Resolve fifo_ValidRegs simpleFifo_ValidRegs.
+Hint Resolve fifo_ModEquiv simpleFifo_ModEquiv
+     debugFifo_ModEquiv debugFifoN_ModEquiv.
+Hint Resolve fifo_ValidRegs simpleFifo_ValidRegs
+     debugFifo_ValidRegs debugFifoN_ValidRegs.
